src/HOL/Theorie.v
@@ -9,50 +9,50 @@ Import ListNotations.
 
 Require Import CRM.Prelude.ListCRM.
 
-Definition proof_ctx (n : nat) (Γ : HOL_ctx n) := list (tm n).
+Definition proof_ctx (n : nat) := list (tm n).
 
-Definition wt_ctx {n : nat} {Γ : HOL_ctx n} (Ξ : proof_ctx n Γ) : Prop :=
+Definition wt_ctx {n : nat} (Γ : HOL_ctx n) (Ξ : proof_ctx n) : Prop :=
   forall_l (fun Θ => Γ ⊢⟨ n ⟩ Θ ~: ℙₛ) Ξ.
 
 Inductive proving : forall (n : nat) (Γ : HOL_ctx n)
-                           (Ξ : proof_ctx n Γ) (φ : tm n), Prop :=
+                           (Ξ : proof_ctx n) (φ : tm n), Prop :=
 | pr_ax : forall {n : nat} {Γ : HOL_ctx n}
-                 {Ξ : proof_ctx n Γ} {φ : tm n},
-    wt_ctx Ξ -> In φ Ξ -> proving n Γ Ξ φ
+                 {Ξ : proof_ctx n} {φ : tm n},
+    wt_ctx Γ Ξ -> In φ Ξ -> proving n Γ Ξ φ
 | pr_transp : forall {n : nat} {Γ : HOL_ctx n}
-                     {Ξ : proof_ctx n Γ} (φ : tm n)
+                     {Ξ : proof_ctx n} (φ : tm n)
                      {ψ : tm n},
     proving n Γ Ξ φ -> Γ ⊢⟨ n ⟩ ψ ~: ℙₛ ->
     φ =ₛ ψ -> proving n Γ Ξ ψ
 | pr_abs : forall {n : nat} {Γ : HOL_ctx n}
-                  {Ξ : proof_ctx n Γ} {φ ψ : tm n},
+                  {Ξ : proof_ctx n} {φ ψ : tm n},
     proving n Γ (φ :: Ξ) ψ -> proving n Γ Ξ (φ ⇒ₛ ψ)
 | pr_app : forall {n : nat} {Γ : HOL_ctx n}
-                  {Ξ : proof_ctx n Γ} (φ : tm n)
+                  {Ξ : proof_ctx n} (φ : tm n)
                   {ψ : tm n},
     proving n Γ Ξ (φ ⇒ₛ ψ) -> proving n Γ Ξ φ ->
     proving n Γ Ξ ψ
-| pr_abs_f : forall {n : nat} {Γ : HOL_ctx n} {Ξ : proof_ctx n Γ}
+| pr_abs_f : forall {n : nat} {Γ : HOL_ctx n} {Ξ : proof_ctx n}
                     {φ : tm (S n)} {s : st},
     proving (S n) (s .: Γ) (List.map (ren_tm shift) Ξ) φ ->
     proving n Γ Ξ (∀ₛ s φ)
-| pr_app_f : forall {n : nat} {Γ : HOL_ctx n} {Ξ : proof_ctx n Γ}
+| pr_app_f : forall {n : nat} {Γ : HOL_ctx n} {Ξ : proof_ctx n}
                     {φ : tm (S n)} (t : tm n) (s : st),
     proving n Γ Ξ (∀ₛ s φ) -> Γ ⊢⟨ n ⟩ t ~: s ->
     proving n Γ Ξ (φ [t .: (fun v => ⟦ v ⟧ₛ)])
-| pr_recN : forall {n : nat} {Γ : HOL_ctx n} {Ξ : proof_ctx n Γ}
+| pr_recN : forall {n : nat} {Γ : HOL_ctx n} {Ξ : proof_ctx n}
                    {φ : tm n},
     proving n Γ Ξ (φ @ₛ Zₛ) ->
     proving n Γ Ξ
       (∀ₛ ℕₛ ((ren_tm shift φ @ₛ ((S n) __tm var_zero)) ⇒ₛ
                 (ren_tm shift φ @ₛ (Sₛ ((S n) __tm var_zero))))) ->
     proving n Γ Ξ (∀ₛ ℕₛ (ren_tm shift φ @ₛ ((S n) __tm var_zero)))
-| pr_recB : forall {n : nat} {Γ : HOL_ctx n} {Ξ : proof_ctx n Γ}
+| pr_recB : forall {n : nat} {Γ : HOL_ctx n} {Ξ : proof_ctx n}
                    {φ : tm n},
     proving n Γ Ξ (φ @ₛ ttₛ) ->
     proving n Γ Ξ (φ @ₛ ffₛ) ->
     proving n Γ Ξ (∀ₛ 𝔹ₛ (ren_tm shift φ @ₛ ((S n) __tm var_zero)))
-| pr_recL : forall {n : nat} {Γ : HOL_ctx n} {Ξ : proof_ctx n Γ}
+| pr_recL : forall {n : nat} {Γ : HOL_ctx n} {Ξ : proof_ctx n}
                    {s : st} {φ : tm n},
     proving n Γ Ξ (φ @ₛ []ₛ) ->
     proving n Γ Ξ
@@ -61,69 +61,144 @@ Inductive proving : forall (n : nat) (Γ : HOL_ctx n)
           (ren_tm (shift >> shift) φ @ₛ
              (((S (S n)) __tm (shift var_zero)) ::ₛ
              ((S (S n)) __tm var_zero))))) ->
-    proving n Γ Ξ (∀ₛ (𝕃ₛ s) (ren_tm shift φ @ₛ ((S n) __tm var_zero))).
+    proving n Γ Ξ (∀ₛ (𝕃ₛ s) (ren_tm shift φ @ₛ ((S n) __tm var_zero)))
+| pr_sort_Z : forall {n : nat} {Γ : HOL_ctx n} {Ξ : proof_ctx n},
+    wt_ctx Γ Ξ -> proving n Γ Ξ (𝕊 ℕₛ Zₛ)
+| pr_sort_S : forall {n : nat} {Γ : HOL_ctx n} {Ξ : proof_ctx n}
+                     {t : tm n},
+    proving n Γ Ξ (𝕊 ℕₛ t) -> proving n Γ Ξ (𝕊 ℕₛ (Sₛ t))
+| pr_sort_recN : forall {n : nat} {Γ : HOL_ctx n} {Ξ : proof_ctx n}
+                        {t u v : tm n} {s : st},
+    proving n Γ Ξ (𝕊 s t) -> proving n Γ Ξ (𝕊 (ℕₛ →ₛ s →ₛ s) u) ->
+    proving n Γ Ξ (𝕊 ℕₛ v) -> proving n Γ Ξ (𝕊 s (recℕₛ t u v))
+| pr_sort_T : forall {n : nat} {Γ : HOL_ctx n} {Ξ : proof_ctx n},
+    wt_ctx Γ Ξ -> proving n Γ Ξ (𝕊 𝔹ₛ ttₛ)
+| pr_sort_F : forall {n : nat} {Γ : HOL_ctx n} {Ξ : proof_ctx n},
+    wt_ctx Γ Ξ -> proving n Γ Ξ (𝕊 𝔹ₛ ffₛ)
+| pr_sort_recB : forall {n : nat} {Γ : HOL_ctx n} {Ξ : proof_ctx n}
+                        {t u v : tm n} {s : st},
+    proving n Γ Ξ (𝕊 s t) -> proving n Γ Ξ (𝕊 s u) ->
+    proving n Γ Ξ (𝕊 𝔹ₛ v) -> proving n Γ Ξ (𝕊 s (rec𝔹ₛ t u v))
+| pr_sort_nil : forall {n : nat} {Γ : HOL_ctx n} {Ξ : proof_ctx n}
+                       {s : st},
+    wt_ctx Γ Ξ -> proving n Γ Ξ (𝕊 (𝕃ₛ s) []ₛ)
+| pr_sort_cons : forall {n : nat} {Γ : HOL_ctx n} {Ξ : proof_ctx n}
+                        {t u : tm n} {s : st},
+    proving n Γ Ξ (𝕊 s t) -> proving n Γ Ξ (𝕊 (𝕃ₛ s) u) ->
+    proving n Γ Ξ (𝕊 (𝕃ₛ s) (t ::ₛ u))
+| pr_sort_recL : forall {n : nat} {Γ : HOL_ctx n} {Ξ : proof_ctx n}
+                        {t u v : tm n} {s : st} (s' : st),
+    proving n Γ Ξ (𝕊 s t) -> proving n Γ Ξ (𝕊 (s' →ₛ 𝕃ₛ s' →ₛ s →ₛ s) u) ->
+    proving n Γ Ξ (𝕊 (𝕃ₛ s') v) -> proving n Γ Ξ (𝕊 s (rec𝕃ₛ t u v))
+| pr_sort_lam : forall {n : nat} {Γ : HOL_ctx n} {Ξ : proof_ctx n}
+                       {t : tm (S n)} {s s' : st},
+    proving (S n) (s .: Γ) ((𝕊 s ⟦ var_zero ⟧ₛ) :: map (ren_tm shift) Ξ) (𝕊 s' t) ->
+    proving n Γ Ξ (𝕊 (s →ₛ s') (ƛ t))
+| pr_sort_app : forall {n : nat} {Γ : HOL_ctx n} {Ξ : proof_ctx n}
+                       {t u : tm n} (s : st) {s' : st},
+    proving n Γ Ξ (𝕊 (s →ₛ s') t) -> proving n Γ Ξ (𝕊 s u) ->
+    proving n Γ Ξ (𝕊 s' (t @ₛ u))
+| pr_sort_pair : forall {n : nat} {Γ : HOL_ctx n} {Ξ : proof_ctx n}
+                        {t u : tm n} {s s' : st},
+    proving n Γ Ξ (𝕊 s t) -> proving n Γ Ξ (𝕊 s' u) ->
+    proving n Γ Ξ (𝕊 (s ×ₛ s') ⟨ t , u ⟩ₛ)
+| pr_sort_proj1 : forall {n : nat} {Γ : HOL_ctx n} {Ξ : proof_ctx n}
+                         {t : tm n} {s : st} (s' : st),
+    proving n Γ Ξ (𝕊 (s ×ₛ s') t) -> proving n Γ Ξ (𝕊 s (π¹ₛ t))
+| pr_sort_proj2 : forall {n : nat} {Γ : HOL_ctx n} {Ξ : proof_ctx n}
+                         {t : tm n} (s : st) {s' : st},
+    proving n Γ Ξ (𝕊 (s ×ₛ s') t) -> proving n Γ Ξ (𝕊 s' (π²ₛ t)).
 
 Notation "Γ ∣ Ξ ⊢| n | φ" := (proving n Γ Ξ φ) (at level 87).
 
 Lemma wt_proving :
-  forall (n : nat) (Γ : HOL_ctx n) (Ξ : proof_ctx n Γ) (φ : tm n),
-    Γ ∣ Ξ ⊢| n | φ -> wt_ctx Ξ /\ (Γ ⊢⟨ n ⟩ φ ~: ℙₛ).
+  forall (n : nat) (Γ : HOL_ctx n) (Ξ : proof_ctx n) (φ : tm n),
+    Γ ∣ Ξ ⊢| n | φ -> wt_ctx Γ Ξ /\ (Γ ⊢⟨ n ⟩ φ ~: ℙₛ).
 Proof.
-  intros. induction H.
-  - split. apply H.
-    apply (In_forall _ Ξ φ H H0).
-  - destruct IHproving as [wtΞ wtφ].
-    split ; [exact wtΞ | exact H0 ].
-  - destruct IHproving as [wtφΞ wtψ].
-    split; [exact (forall_tail _ _ _ wtφΞ) |].
-    constructor. apply (forall_head _ _ _ wtφΞ).
-    apply wtψ.
-  - destruct IHproving1 as [wtΞ wtψ].
-    dependent destruction wtψ. split. apply wtΞ.
-    apply wtψ2.
-  - destruct IHproving. split.
-    + clear φ H H1.
-      apply (map_forall_rev _ _ (ren_tm shift)
-               (fun x => typ_weaken_rev n Γ x ℙₛ _)) in H0.
-      apply H0.
-    + apply (typ_forall s). apply H1.
-  - destruct IHproving. split. apply H1.
-    apply (comp_typ_vec _ _ _ _ (s .: Γ)).
+  intros. induction H; try (split; [assumption | ]);
+    try (destruct IHproving as [HΞ IH]; split; [try assumption | try assumption]);
+    try (destruct IHproving1 as [HΞ IH1]; destruct IHproving2 as [_ IH2];
+         try destruct IHproving3 as [_ IH3];
+         split; [try assumption| try assumption]);
+    try (constructor; constructor; fail).
+  - apply (In_forall _ Ξ φ H H0).
+  - dependent destruction HΞ. apply HΞ.
+  - constructor; [| assumption]. inversion HΞ.
+    apply H2.
+  - dependent destruction IH1. apply IH1_2.
+  - eapply (map_forall_rev _
+              (fun x => s .: Γ ⊢⟨ S n ⟩ x ~: ℙₛ)
+              (ren_tm shift)).
+    intros a Ha.
+    eapply typ_weaken_rev.
+    apply Ha. apply HΞ.
+  - apply typ_forall. apply IH.
+  - apply (comp_typ_vec _ _ _ _ (s .: Γ)).
     asimpl. intro f; case f eqn:e.
     asimpl. apply typ_var. asimpl. apply H0.
-    dependent destruction H2. apply H2.
-  - destruct IHproving1 as [H1 H2]. split; [apply H1|].
-    constructor. apply (typ_app ℕₛ).
-    apply typ_weaken. dependent destruction H2.
-    dependent destruction H2_0. apply H2_.
+    dependent destruction IH. apply IH.
+  - constructor. apply (typ_app ℕₛ).
+    apply typ_weaken. dependent destruction IH1.
+    dependent destruction IH1_2. apply IH1_1.
     constructor.
-  - destruct IHproving1 as [H1 H2]. split; [apply H1|].
-    constructor. apply (typ_app 𝔹ₛ).
-    apply typ_weaken. dependent destruction H2.
-    dependent destruction H2_0. apply H2_.
+  - constructor. apply (typ_app 𝔹ₛ).
+    apply typ_weaken. dependent destruction IH2.
+    dependent destruction IH2_2. apply IH2_1.
     constructor.
-  - destruct IHproving1 as [H1 H2]. split; [apply H1|].
-    constructor. apply (typ_app (𝕃ₛ s)).
-    apply typ_weaken. dependent destruction H2.
-    dependent destruction H2_0.
-    destruct IHproving2 as [_ H3].
-    dependent destruction H3. dependent destruction H3.
-    dependent destruction H3.
-    dependent destruction H3_0.
-    dependent destruction H3_0_1.
-    simpl in H3_.
-    assert (ren_tm (shift >> shift) φ =
-              ren_tm shift (ren_tm shift φ)).
-    asimpl; reflexivity.
-    apply (typ_weaken_rev _ _ _ _ s).
-    apply (typ_weaken_rev _ _ _ _ (𝕃ₛ s)).
-    asimpl. apply H3_.
-    constructor.
+  - constructor. apply (typ_app (𝕃ₛ s)).
+    apply typ_weaken. dependent destruction IH2.
+    dependent destruction IH2.
+    dependent destruction IH2.
+    dependent destruction IH2_2.
+    dependent destruction IH2_2_2.
+    apply (typ_weaken_rev _ _ _ _ s0).
+    apply (typ_weaken_rev _ _ _ _ (𝕃ₛ s0)).
+    asimpl. apply IH2_1. constructor.
+  - constructor. dependent destruction IH.
+    constructor. apply IH.
+  - constructor. dependent destruction IH1.
+    dependent destruction IH2.
+    dependent destruction IH3.
+    constructor; assumption.
+  - dependent destruction IH1.
+    dependent destruction IH2.
+    dependent destruction IH3.
+    constructor. constructor; assumption.
+  - dependent destruction IH1.
+    dependent destruction IH2.
+    constructor. constructor; assumption.
+  - dependent destruction IH1.
+    dependent destruction IH2.
+    dependent destruction IH3.
+    constructor. apply (typ_recL s'); assumption.
+  - dependent destruction HΞ.
+    eapply (map_forall_rev _
+              (fun x => s .: Γ ⊢⟨ S n ⟩ x ~: ℙₛ)
+              (ren_tm shift)).
+    intros a Ha.
+    eapply typ_weaken_rev.
+    apply Ha.
+    apply HΞ.
+  - constructor. constructor.
+    dependent destruction IH.
+    apply IH.
+  - constructor.
+    dependent destruction IH1.
+    dependent destruction IH2.
+    apply (typ_app s); assumption.
+  - constructor.
+    dependent destruction IH1.
+    dependent destruction IH2.
+    constructor; assumption.
+  - constructor. dependent destruction IH.
+    apply (typ_proj1 s'). assumption.
+  - constructor. dependent destruction IH.
+    apply (typ_proj2 s). assumption.
 Qed.
 
 Lemma ren_proof :
   forall (n m : nat) (Γ : HOL_ctx n) (Δ : HOL_ctx m)
-         (Ξ : proof_ctx n Γ) (φ : tm n) (ξ : fin n -> fin m),
+         (Ξ : proof_ctx n) (φ : tm n) (ξ : fin n -> fin m),
     (forall f, (ξ >> Δ) f = Γ f) ->
     Γ ∣ Ξ ⊢| n | φ -> Δ ∣ map (ren_tm ξ) Ξ ⊢| m | ren_tm ξ φ.
 Proof.
@@ -182,11 +257,88 @@ Proof.
     unfold ">>" in IHproving2.
     asimpl in IHproving2.
     apply IHproving2.
+  - apply pr_sort_Z.
+    apply (map_forall (fun x => Γ ⊢⟨ n ⟩ x ~: ℙₛ)
+             (fun x => Δ ⊢⟨ m ⟩ x ~: ℙₛ)
+             (ren_tm ξ)).
+    intros a Ha.
+    eapply typ_ren.
+    apply H0. apply Ha.
+    apply H.
+  - apply pr_sort_S.
+    apply IHproving. apply H.
+  - apply pr_sort_recN.
+    apply IHproving1; assumption.
+    apply IHproving2; assumption.
+    apply IHproving3; assumption.
+  - apply pr_sort_T.
+    apply (map_forall (fun x => Γ ⊢⟨ n ⟩ x ~: ℙₛ)
+             (fun x => Δ ⊢⟨ m ⟩ x ~: ℙₛ)
+             (ren_tm ξ)).
+    intros a Ha.
+    eapply typ_ren.
+    apply H0. apply Ha.
+    apply H.
+  - apply pr_sort_F.
+    apply (map_forall (fun x => Γ ⊢⟨ n ⟩ x ~: ℙₛ)
+             (fun x => Δ ⊢⟨ m ⟩ x ~: ℙₛ)
+             (ren_tm ξ)).
+    intros a Ha.
+    eapply typ_ren.
+    apply H0. apply Ha.
+    apply H.
+  - apply pr_sort_recB.
+    apply IHproving1; assumption.
+    apply IHproving2; assumption.
+    apply IHproving3; assumption.
+  - apply pr_sort_nil.
+    apply (map_forall (fun x => Γ ⊢⟨ n ⟩ x ~: ℙₛ)
+             (fun x => Δ ⊢⟨ m ⟩ x ~: ℙₛ)
+             (ren_tm ξ)).
+    intros a Ha.
+    eapply typ_ren.
+    apply H0. apply Ha.
+    apply H.
+  - apply pr_sort_cons.
+    apply IHproving1; assumption.
+    apply IHproving2; assumption.
+  - apply (pr_sort_recL s').
+    apply IHproving1; assumption.
+    apply IHproving2; assumption.
+    apply IHproving3; assumption.
+  - apply pr_sort_lam.
+    specialize (IHproving (S m) (s .: Δ) (upRen_tm_tm ξ)).
+    asimpl in IHproving.
+    assert
+      (forall f, ((var_zero .: ξ >> shift) >> (s .: Δ)) f = (s .: Γ) f).
+    intro f; case f eqn : e. asimpl.
+    unfold ">>"; simpl. apply H. reflexivity.
+    specialize (IHproving H1); clear H1.
+    asimpl in IHproving. simpl in IHproving.
+    rewrite map_map in IHproving.
+    asimpl in IHproving.
+    rewrite map_map. asimpl.
+    assert (forall f,
+               (ren_tm shift >> ren_tm (var_zero .: ξ >> shift)) f =
+                 (ren_tm ξ >> ren_tm shift) f).
+    intro f; asimpl. reflexivity.
+    rewrite (map_ext _ _ H1) in IHproving.
+    apply IHproving.
+  - apply (pr_sort_app s).
+    apply IHproving1; assumption.
+    apply IHproving2; assumption.
+  - apply pr_sort_pair.
+    apply IHproving1; assumption.
+    apply IHproving2; assumption.
+  - apply (pr_sort_proj1 s').
+    apply IHproving; assumption.
+  - apply (pr_sort_proj2 s).
+    apply IHproving; assumption.
 Qed.
 
 Lemma subst_proof :
   forall (n m : nat) (v : HOL_vec n m) (Γ : HOL_ctx m) (Δ : HOL_ctx n)
-         (Ξ : proof_ctx n Δ) (φ : tm n),
+         (Ξ : proof_ctx n) (φ : tm n),
     Γ ⊢⟨ m ⟩ v ~:⟨ n , Δ ⟩ -> Δ ∣ Ξ ⊢| n | φ ->
     Γ ∣ map (subst_tm v) Ξ ⊢| m | φ [ v ].
 Proof.
@@ -255,13 +407,93 @@ Proof.
     rewrite H in IHHφ2; clear H.
     specialize (pr_recL IHHφ1 IHHφ2).
     asimpl. trivial.
+  - apply pr_sort_Z.
+    apply (map_forall
+             (fun x => Γ  ⊢⟨ n ⟩ x ~: ℙₛ)
+             (fun x => Γ0 ⊢⟨ m ⟩ x ~: ℙₛ)
+             (subst_tm v)).
+    intros a Ha.
+    apply (comp_typ_vec _ _ _ _ _ _ _ Hv Ha).
+    apply H.
+  - asimpl. apply pr_sort_S.
+    apply IHHφ.
+    apply Hv.
+  - asimpl. apply pr_sort_recN.
+    apply IHHφ1; assumption.
+    apply IHHφ2; assumption.
+    apply IHHφ3; assumption.
+  - apply pr_sort_T.
+    apply (map_forall
+             (fun x => Γ  ⊢⟨ n ⟩ x ~: ℙₛ)
+             (fun x => Γ0 ⊢⟨ m ⟩ x ~: ℙₛ)
+             (subst_tm v)).
+    intros a Ha.
+    apply (comp_typ_vec _ _ _ _ _ _ _ Hv Ha).
+    apply H.
+  - apply pr_sort_F.
+    apply (map_forall
+             (fun x => Γ  ⊢⟨ n ⟩ x ~: ℙₛ)
+             (fun x => Γ0 ⊢⟨ m ⟩ x ~: ℙₛ)
+             (subst_tm v)).
+    intros a Ha.
+    apply (comp_typ_vec _ _ _ _ _ _ _ Hv Ha).
+    apply H.
+  - asimpl. apply pr_sort_recB.
+    apply IHHφ1; assumption.
+    apply IHHφ2; assumption.
+    apply IHHφ3; assumption.
+  - apply pr_sort_nil.
+    apply (map_forall
+             (fun x => Γ  ⊢⟨ n ⟩ x ~: ℙₛ)
+             (fun x => Γ0 ⊢⟨ m ⟩ x ~: ℙₛ)
+             (subst_tm v)).
+    intros a Ha.
+    apply (comp_typ_vec _ _ _ _ _ _ _ Hv Ha).
+    apply H.
+  - asimpl. apply pr_sort_cons.
+    apply IHHφ1; assumption.
+    apply IHHφ2; assumption.
+  - asimpl. apply (pr_sort_recL s').
+    apply IHHφ1; assumption.
+    apply IHHφ2; assumption.
+    apply IHHφ3; assumption.
+  - asimpl. apply pr_sort_lam.
+    specialize (IHHφ (S m) ((S m)__tm var_zero .: v >> ren_tm shift)
+                  (s .: Γ0)).
+    assert (s .: Γ0 ⊢⟨ S m ⟩ (S m) __tm var_zero .: v >> ren_tm shift ~:⟨ S n, s .: Γ ⟩).
+    intro f. case f eqn : e.
+    asimpl. unfold ">>". apply typ_weaken. apply Hv.
+    asimpl. constructor.
+    specialize (IHHφ H); clear H.
+    asimpl in IHHφ.
+    rewrite map_map. asimpl.
+    simpl in IHHφ. rewrite map_map in IHHφ.
+    asimpl in IHHφ.
+    assert
+      (forall f,
+          (ren_tm shift >> subst_tm
+             ((S m)__tm var_zero .: v >> ren_tm shift)) f =
+            (subst_tm v >> ren_tm shift) f).
+    intro f; asimpl. reflexivity.
+    rewrite (map_ext _ _ H) in IHHφ.
+    apply IHHφ.
+  - asimpl. apply (pr_sort_app s).
+    apply IHHφ1; assumption.
+    apply IHHφ2; assumption.
+  - asimpl. apply pr_sort_pair.
+    apply IHHφ1; assumption.
+    apply IHHφ2; assumption.
+  - asimpl. apply (pr_sort_proj1 s').
+    apply IHHφ; assumption.
+  - asimpl. apply (pr_sort_proj2 s).
+    apply IHHφ; assumption.
 Qed.
 
 Lemma weaken_proof :
   forall (n : nat) (Γ : HOL_ctx n)
-         (Ξ Θ : proof_ctx n Γ) (φ : tm n),
+         (Ξ Θ : proof_ctx n) (φ : tm n),
     Γ ∣ Ξ ⊢| n | φ -> incl Ξ Θ ->
-    wt_ctx Θ -> Γ ∣ Θ ⊢| n | φ.
+    wt_ctx Γ Θ -> Γ ∣ Θ ⊢| n | φ.
 Proof.
   intros; revert Θ H0 H1; induction H; intros.
   - apply pr_ax. apply H2. apply H1.
@@ -298,11 +530,55 @@ Proof.
     apply IHproving2. apply H1. apply H2.
   - apply pr_recL. apply IHproving1. apply H1. apply H2.
     apply IHproving2. apply H1. apply H2.
+  - apply pr_sort_Z; assumption.
+  - apply pr_sort_S. apply IHproving; assumption.
+  - apply pr_sort_recN.
+    apply IHproving1; assumption.
+    apply IHproving2; assumption.
+    apply IHproving3; assumption.
+  - apply pr_sort_T; assumption.
+  - apply pr_sort_F; assumption.
+  - apply pr_sort_recB.
+    apply IHproving1; assumption.
+    apply IHproving2; assumption.
+    apply IHproving3; assumption.
+  - apply pr_sort_nil; assumption.
+  - apply pr_sort_cons.
+    apply IHproving1; assumption.
+    apply IHproving2; assumption.
+  - apply (pr_sort_recL s').
+    apply IHproving1; assumption.
+    apply IHproving2; assumption.
+    apply IHproving3; assumption.
+  - apply pr_sort_lam. apply IHproving.
+    apply incl_cons.
+    left; reflexivity.
+    apply incl_tl.
+    apply incl_map. apply H0.
+    constructor.
+    constructor. constructor.
+    apply (map_forall
+             (fun x => Γ  ⊢⟨ n ⟩ x ~: ℙₛ)
+             (fun x => s .: Γ ⊢⟨ S n ⟩ x ~: ℙₛ)
+             (ren_tm shift)).
+    intros a Ha. apply typ_weaken.
+    apply Ha.
+    apply H1.
+  - apply (pr_sort_app s).
+    apply IHproving1; assumption.
+    apply IHproving2; assumption.
+  - apply pr_sort_pair.
+    apply IHproving1; assumption.
+    apply IHproving2; assumption.
+  - apply (pr_sort_proj1 s').
+    apply IHproving; assumption.
+  - apply (pr_sort_proj2 s).
+    apply IHproving; assumption.
 Qed.
 
 Lemma weaken_proof_1 :
   forall (n : nat) (Γ : HOL_ctx n)
-         (Ξ : proof_ctx n Γ) (φ ψ : tm n),
+         (Ξ : proof_ctx n) (φ ψ : tm n),
     Γ ∣ Ξ ⊢| n | φ -> Γ ⊢⟨ n ⟩ ψ ~: ℙₛ ->
     Γ ∣ ψ :: Ξ ⊢| n | φ.
 Proof.
